#+OPTIONS: toc:nil

\noindent\textbf{Exercise 1.19}: Taking successive applications of $T_{pq}$ gives us
\begin{align*}
        T^2_{pq} &= T_{pq}\bigl(T_{pq}(a,b)\bigr) = T_{pq}\bigl(bq + aq + ap, bp + aq\bigr) \\
                 &= \Bigl((bp + aq)q + (bq + aq + ap)q + (bq + aq + ap)p, (bp + aq)p + (bq + aq + ap)q\Bigr).
\end{align*}
Now consider the second value in the tuple, we have that
\begin{align*}
        (bp + aq)q + (bq + aq + ap)q = b(p^2 + q^2) + a(2pq + q^2),
\end{align*}
which gives us $p' = (p^2 + q^2)$ and $q' = (q^2 + 2pq)$. Then
\begin{align*}
        bq' + aq' + ap' &= b(q^2 + 2pq) + a(q^2 + 2pq) + a(p^2 + q^2) \\
                        &= bq^2 + 2bpq + aq^2 + 2apq + ap^2 + aq^2 = \\
                        &= (bp + aq)q + (bq + aq + ap)q + (bq + aq + ap)p,
\end{align*}
which is the first value in the tuple. Thus,
\begin{align*}
        T^2_{pq}(a,b) &= \bigl(bq' + aq' + ap', bp' + aq'\bigr).
\end{align*}
\hfill$\square$
